Finished clocking preservation proof

src/Lustre/Normalization/NClocking.v
@@ -229,10 +229,35 @@ Module Type NCLOCKING
     repeat rewrite nclocksof_annots. congruence.
   Qed.
 
+  Fact normalize_rhs_nclockof : forall G vars e keep_fby es' eqs' st st',
+      wc_exp G vars e ->
+      normalize_rhs keep_fby e st = (es', eqs', st') ->
+      nclocksof es' = nclockof e.
+  Proof with eauto.
+    intros.
+    eapply normalize_rhs_annot in H0; eauto.
+    rewrite nclocksof_annots, H0, <- nclockof_annot. reflexivity.
+  Qed.
+
+  Fact normalize_rhss_nclocksof : forall G vars es keep_fby es' eqs' st st',
+      Forall (wc_exp G vars) es ->
+      normalize_rhss keep_fby es st = (es', eqs', st') ->
+      nclocksof es' = nclocksof es.
+  Proof with eauto.
+    intros.
+    eapply normalize_rhss_annots in H0; eauto.
+    rewrite nclocksof_annots, H0, <- nclocksof_annots. reflexivity.
+  Qed.
+
   (** ** A few additional things *)
 
   Definition st_clocks (st : fresh_st ((Op.type * clock) * bool)) :=
-    List.map (fun '(id, ((_, cl), _)) => (id, cl)) (st_anns st).
+    idck (idty (st_anns st)).
+
+  Local Ltac In_st_clocks id t cl b :=
+    unfold st_clocks, idck, idty in *;
+    repeat simpl_In; exists (id, (t, cl)); split; auto;
+    simpl_In; exists (id, (t, cl, b)); eauto.
 
   Fact idents_for_anns_incl_clocks : forall anns ids st st',
     idents_for_anns anns st = (ids, st') ->
@@ -245,9 +270,7 @@ Module Type NCLOCKING
     specialize (Hids (id, (t, cl))).
     assert (In (id, (t, cl)) (idty (st_anns st'))).
     { eapply Hids. repeat simpl_In. exists (id, (t, (cl, o))); auto. }
-    unfold st_clocks, idty in *.
-    repeat simpl_In. inv H.
-    exists (id, (t, cl, b)); auto.
+    In_st_clocks id t cl b. inv H; auto.
   Qed.
 
   Fact idents_for_anns'_incl_clocks : forall anns ids st st',
@@ -261,16 +284,14 @@ Module Type NCLOCKING
     specialize (Hids (id, (t, cl))).
     assert (In (id, (t, cl)) (idty (st_anns st'))).
     { eapply Hids. repeat simpl_In. exists (id, (t, (cl, o))); auto. }
-    unfold st_clocks, idty in *.
-    repeat simpl_In. inv H.
-    exists (id, (t, cl, b)); auto.
+    In_st_clocks id t cl b. inv H; auto.
   Qed.
 
   Fact idents_for_anns'_clocknames : forall anns ids st st',
       idents_for_anns' anns st = (ids, st') ->
       Forall (fun x => LiftO True (eq (fst x)) (snd (snd (snd x)))) ids.
   Proof with eauto.
-    induction anns; intros ids st st' Hids; simpl in *; repeat inv_bind...
+    induction anns; intros ids st st' Hids; repeat inv_bind...
     destruct a as [ty [cl [name|]]]; repeat inv_bind; constructor; simpl...
   Qed.
 
@@ -308,39 +329,187 @@ Module Type NCLOCKING
       eapply incl_map; eauto
     end; auto.
 
-  (** ** For a normalized_lexp, wc_exp implies wc_clock (clockof) *)
+  (** ** Auxilary lemmas for perservation of wc_env *)
 
-  Lemma wc_exp_clockof : forall G vars e,
-      normalized_lexp e ->
-      wc_env vars ->
-      wc_exp G vars e ->
-      Forall (wc_clock vars) (clockof e).
-  Proof with eauto.
-    intros G e vas Hnormed Henv Hwc.
-    induction Hnormed; inv Hwc; simpl; unfold clock_of_nclock, stripname;
-      simpl in *; repeat constructor...
-    - (* var *)
-      unfold wc_env in Henv; rewrite Forall_forall in Henv.
-      apply Henv in H0...
-    - (* var (anon) *)
-      unfold wc_env in Henv; rewrite Forall_forall in Henv.
-      apply Henv in H0...
-    - (* unop *)
-      apply IHHnormed in H1...
-      rewrite H4 in H1. inv H1...
-    - (* binop *)
-      apply IHHnormed1 in H3...
-      rewrite H6 in H3. inv H3...
-    - (* when *)
-      inv H3; clear H2.
-      apply IHHnormed in H1.
-      rewrite app_nil_r in *. symmetry in H7. singleton_length.
-      inv H6. inv H1...
+  Import Permutation.
+
+  Fact fresh_ident_wc_env : forall vars ty ck b id st st',
+      wc_env (vars++st_clocks st) ->
+      wc_clock (vars++st_clocks st) ck ->
+      fresh_ident ((ty, ck), b) st = (id, st') ->
+      wc_env (vars++st_clocks st').
+  Proof.
+    intros vars ty ck b id st st' Hwenv Hwc Hfresh.
+    apply fresh_ident_anns in Hfresh.
+    unfold st_clocks in *. rewrite Hfresh; simpl.
+    rewrite <- Permutation_middle.
+    constructor; simpl.
+    - repeat solve_incl.
+    - eapply Forall_impl; [|eauto].
+      intros; simpl in *. repeat solve_incl.
   Qed.
 
-  (** ** Perservation of wc_env *)
+  Fact idents_for_anns_wc_env : forall vars anns ids st st',
+      wc_env (vars++st_clocks st) ->
+      Forall (wc_clock (vars++st_clocks st)) (map fst (map snd anns)) ->
+      idents_for_anns anns st = (ids, st') ->
+      wc_env (vars++st_clocks st').
+  Proof with eauto.
+    induction anns as [|[ty [ck id]]]; intros ids st st' Hwenv Hwc Hids;
+      repeat inv_bind...
+    inv Hwc.
+    eapply IHanns in H0... 2:(solve_forall; repeat solve_incl).
+    eapply fresh_ident_wc_env...
+  Qed.
 
-  (* Fact normalize_exp_wc_env : forall *)
+  Fact reuse_ident_wc_env : forall vars ty ck b id st st',
+      wc_env (vars++st_clocks st) ->
+      wc_clock (vars++st_clocks st') ck ->
+      reuse_ident id ((ty, ck), b) st = (tt, st') ->
+      wc_env (vars++st_clocks st').
+  Proof.
+    intros vars ty ck b id st st' Hwenv Hwc Hfresh.
+    apply reuse_ident_anns in Hfresh.
+    unfold st_clocks in *. rewrite Hfresh; simpl.
+    rewrite <- Permutation_middle.
+    constructor; simpl.
+    - solve_incl. rewrite Hfresh; simpl.
+      rewrite Permutation_middle. apply incl_refl.
+    - eapply Forall_impl; [|eauto].
+      intros; simpl in *. repeat solve_incl.
+  Qed.
+
+  Fact idents_for_anns'_st_anns : forall anns ids st st',
+      idents_for_anns' anns st = (ids, st') ->
+      Permutation (idty (st_anns st')) (map (fun '(id, (ty, (cl, _))) => (id, (ty, cl))) ids++idty (st_anns st)).
+  Proof with eauto.
+    induction anns; intros ids st st' Hids;
+      repeat inv_bind; simpl in *...
+    destruct a as [ty [cl [name|]]]; repeat inv_bind; simpl in *.
+    - rewrite IHanns...
+      rewrite Permutation_middle. apply Permutation_app_head.
+      destruct x. apply reuse_ident_anns in H.
+      rewrite H. reflexivity.
+    - rewrite IHanns...
+      rewrite Permutation_middle. apply Permutation_app_head.
+      apply fresh_ident_anns in H.
+      rewrite H. reflexivity.
+  Qed.
+
+  Fact idents_for_anns'_wc_env : forall vars anns ids st st',
+      wc_env (vars++st_clocks st) ->
+      Forall (wc_clock (vars++st_clocks st')) (map fst (map snd anns)) ->
+      idents_for_anns' anns st = (ids, st') ->
+      wc_env (vars++st_clocks st').
+  Proof with eauto.
+    intros vars anns ids st st' Hwenv Hwc Hids.
+    specialize (idents_for_anns'_values _ _ _ _ Hids) as Hids'.
+    apply idents_for_anns'_st_anns in Hids.
+    unfold st_clocks. rewrite Hids.
+    unfold st_clocks, idck, idty in *; repeat simpl_list.
+    unfold wc_env in *. repeat rewrite Forall_app in *.
+    destruct Hwenv as [Hwenv1 Hwenv2]. repeat split.
+    - eapply Forall_impl... intros; simpl in *. repeat solve_incl.
+    - clear Hwenv1 Hwenv2.
+      rewrite <- Hids' in Hwc.
+      repeat rewrite Forall_map. repeat rewrite Forall_map in Hwc.
+      eapply Forall_impl...
+      intros [id [ty [cl name]]] ?; simpl in *.
+      intros; simpl in *.
+      solve_incl. apply incl_appr'.
+      replace (map (fun x => (fst x, snd (fst (snd x)))) (st_anns st'))
+                 with (idck (map (fun x => (fst x, fst (snd x))) (st_anns st'))).
+      2:{ unfold idck. rewrite map_map. eapply map_ext. intros [id' [ty' cl']]... }
+      rewrite Hids. unfold idck. rewrite map_app, map_map, map_map.
+      eapply incl_appr', incl_refl.
+    - eapply Forall_impl... intros; simpl in *. repeat solve_incl.
+  Qed.
+
+  Fact init_var_for_clock_wc_env : forall vars cl id eqs' st st',
+      wc_env (vars++st_clocks st) ->
+      wc_clock (vars++st_clocks st) cl ->
+      init_var_for_clock cl st = (id, eqs', st') ->
+      wc_env (vars++st_clocks st').
+  Proof with eauto.
+    intros vars cl id eqs' st st' Hwenv Hwc Hinit.
+    unfold init_var_for_clock in Hinit.
+    destruct find.
+    - destruct p. inv Hinit...
+    - destruct fresh_ident eqn:Hfresh. inv Hinit.
+      eapply fresh_ident_wc_env in Hfresh...
+  Qed.
+
+  Fact fby_iteexp_wc_env : forall vars e0 e ty cl es' eqs' st st',
+      wc_env (vars++st_clocks st) ->
+      wc_clock (vars++st_clocks st) (fst cl) ->
+      fby_iteexp e0 e (ty, cl) st = (es', eqs', st') ->
+      wc_env (vars++st_clocks st').
+  Proof with eauto.
+    intros vars e0 e ty [cl name] es' eqs' st st' Hwenv Hwc Hfby.
+    unfold fby_iteexp in Hfby.
+    destruct (Norm.is_constant e0); repeat inv_bind...
+    eapply fresh_ident_wc_env in H0... 2:repeat solve_incl.
+    eapply init_var_for_clock_wc_env in H...
+  Qed.
+
+  Fact map_bind2_wc_env {A A1 A2 : Type} :
+    forall vars (k : A -> FreshAnn (A1 * A2)) a a1s a2s st st',
+      wc_env (vars++st_clocks st) ->
+      map_bind2 k a st = (a1s, a2s, st') ->
+      (forall st st' a es a2s, k a st = (es, a2s, st') -> st_follows st st') ->
+      Forall (fun a => forall a1s a2s st0 st0',
+                  wc_env (vars++st_clocks st0) ->
+                  k a st0 = (a1s, a2s, st0') ->
+                  st_follows st st0 ->
+                  st_follows st0' st' ->
+                  wc_env (vars++st_clocks st0')) a ->
+      wc_env (vars++st_clocks st').
+  Proof with eauto.
+    induction a; intros a1s a2s st st' Hclocks Hmap Hfollows Hf;
+      simpl in Hmap; repeat inv_bind...
+    inv Hf.
+    specialize (H3 _ _ _ _ Hclocks H).
+    eapply IHa in H3...
+    - reflexivity.
+    - eapply map_bind2_st_follows...
+      solve_forall...
+    - solve_forall.
+      eapply H1 in H2...
+      etransitivity...
+  Qed.
+
+  Fact normalize_fby_wc_env : forall vars e0s es anns es' eqs' st st',
+      wc_env (vars++st_clocks st) ->
+      Forall (fun '(_, (cl, _)) => wc_clock (vars++st_clocks st) cl) anns ->
+      normalize_fby e0s es anns st = (es', eqs', st') ->
+      wc_env (vars++st_clocks st').
+  Proof with eauto.
+    intros vars e0s es anns es' eqs' st st' Hwenv Hwc Hnorm.
+    unfold normalize_fby in Hnorm; repeat inv_bind.
+    eapply map_bind2_wc_env in H...
+    - intros ? ? [[e0 e] ann] ? ? Hfby. repeat solve_st_follows.
+    - clear H.
+      eapply Forall_forall; intros [[e0 e] [ty [cl name]]] ? ? ? ? ? Hwc' Hfby Hfollows1 Hfollows2.
+      eapply fby_iteexp_wc_env in Hfby... simpl.
+      repeat simpl_In. rewrite Forall_forall in Hwc. eapply Hwc in H. repeat solve_incl.
+  Qed.
+
+  Fact normalize_reset_wc_env : forall vars e e' eqs' st st',
+      wc_env (vars++st_clocks st) ->
+      Forall (wc_clock (vars++st_clocks st)) (clockof e) ->
+      normalize_reset e st = (e', eqs', st') ->
+      wc_env (vars++st_clocks st').
+  Proof with eauto.
+    intros vars e e' eqs' st st' Hwenv Hwc Hnorm.
+    specialize (normalize_reset_spec e) as [[v [a [? Hspec]]]|Hspec]; subst;
+      rewrite Hspec in Hnorm; clear Hspec;
+        repeat inv_bind...
+    destruct hd as [ty [cl name]] eqn:Hann; repeat inv_bind.
+    eapply fresh_ident_wc_env in H...
+    rewrite clockof_annot, map_map in Hwc.
+    destruct (annot e) as [|[ty' [cl' name']]]; simpl in *; inv Hann...
+    inv Hwc...
+  Qed.
 
   (** ** Preservation of wc *)
 
@@ -363,7 +532,7 @@ Module Type NCLOCKING
       Forall (wc_exp G (vars++st_clocks st')) (List.map (fun '(x, ann) => Evar x ann) ids).
   Proof.
     induction anns; intros ids st st' Hunnamed Hident;
-      simpl in *; repeat inv_bind; simpl; auto.
+      repeat inv_bind; simpl; auto.
     destruct a as [? [? ?]]. repeat inv_bind.
     inv Hunnamed. constructor; eauto.
     unfold unnamed_stream in H3; simpl in H3; subst.
@@ -372,7 +541,7 @@ Module Type NCLOCKING
     eapply idents_for_anns_st_follows in H0.
     eapply st_follows_incl in H; eauto.
     eapply in_or_app. right.
-    unfold st_clocks. simpl_In. exists (x, (t, c, false)); auto.
+    In_st_clocks x t c false.
   Qed.
 
   Fact idents_for_anns'_wc : forall G vars anns ids st st',
@@ -380,7 +549,7 @@ Module Type NCLOCKING
       Forall (wc_exp G (vars++st_clocks st')) (List.map (fun '(x, ann) => Evar x ann) ids).
   Proof.
     induction anns; intros ids st st' Hident;
-      simpl in *; repeat inv_bind; simpl; auto.
+      repeat inv_bind; simpl; auto.
     destruct a as [? [? ?]].
     destruct o; repeat inv_bind; constructor; eauto.
     - constructor.
@@ -388,13 +557,13 @@ Module Type NCLOCKING
       eapply idents_for_anns'_st_follows in H0.
       eapply st_follows_incl in H; eauto.
       eapply in_or_app. right.
-      unfold st_clocks. simpl_In. exists (i, (t, c, false)); auto.
+      In_st_clocks i t c false.
     - constructor.
       eapply fresh_ident_In in H.
       eapply idents_for_anns'_st_follows in H0.
       eapply st_follows_incl in H; eauto.
       eapply in_or_app. right.
-      unfold st_clocks. simpl_In. exists (x, (t, c, false)); auto.
+      In_st_clocks x t c false.
   Qed.
 
   Fact map_bind2_wc_exp {A A2 B} :
@@ -692,14 +861,13 @@ Module Type NCLOCKING
           eapply fresh_ident_st_follows in H4. eapply st_follows_incl in H4.
           eapply st_follows_incl in H3.
           eapply H4 in H1. eapply H3 in H1; simpl in H1.
-          unfold st_clocks. repeat simpl_In. exists (x, (Op.bool_type, cl, true)); auto.
+          In_st_clocks x Op.bool_type cl true.
         * repeat simpl_In...
           eapply Hwc1 in H10.
           repeat solve_incl.
         * eapply fresh_ident_In in H4; simpl in H4.
           eapply in_or_app. right.
-          unfold st_clocks.
-          repeat simpl_In. exists (x3, (ty, cl, false)); split; auto.
+          In_st_clocks x3 ty cl false.
           eapply st_follows_incl in H3; eauto.
         * rewrite app_nil_r.
           repeat simpl_nth; repeat simpl_length.
@@ -773,8 +941,7 @@ Module Type NCLOCKING
     destruct hd eqn:Hhd, p; repeat inv_bind.
     econstructor. apply fresh_ident_In in H.
     apply in_or_app; right.
-    unfold st_clocks.
-    rewrite in_map_iff. exists (x, (t, c, false)); auto.
+    In_st_clocks x t c false.
   Qed.
 
   Fact normalize_rhs_wc_exp : forall G vars e keep_fby es' eqs' st st',
@@ -817,32 +984,50 @@ Module Type NCLOCKING
         rewrite <- length_clockof_numstreams, H0. reflexivity.
   Qed.
 
-  Fact map_bind2_wc_eq {A A1 B} :
-    forall G vars (k : A -> Fresh (A1 * list equation) B) a a1s eqs' st st',
+  Corollary normalize_rhss_wc_exp : forall G vars es keep_fby es' eqs' st st',
+      Forall (wc_exp G (vars++st_clocks st)) es ->
+      normalize_rhss keep_fby es st = (es', eqs', st') ->
+      Forall (wc_exp G (vars++st_clocks st')) es'.
+  Proof.
+    intros G vars es keep_fby es' eqs' st st' Hwc Hnorm.
+    unfold normalize_rhss in Hnorm; repeat inv_bind.
+    eapply map_bind2_wc_exp in H; eauto.
+    solve_forall.
+    eapply normalize_rhs_wc_exp with (G:=G) (vars:=vars) in H1; eauto.
+    - solve_forall. repeat solve_incl.
+    - repeat solve_incl.
+  Qed.
+
+  Fact map_bind2_wc_eq {A A1} :
+    forall G vars (k : A -> Fresh (A1 * _) _) a a1s eqs' st st',
+      wc_env (vars++st_clocks st) ->
       map_bind2 k a st = (a1s, eqs', st') ->
       (forall st st' a es a2s, k a st = (es, a2s, st') -> st_follows st st') ->
       Forall (fun a => forall a1 eqs' st0 st0',
-                  k a st0 = (a1, eqs', st0') ->
                   st_follows st st0 ->
                   st_follows st0' st' ->
-                  Forall (wc_equation G vars) eqs') a ->
-      Forall (wc_equation G vars) (concat eqs').
-  Proof.
+                  wc_env (vars++st_clocks st0) ->
+                  k a st0 = (a1, eqs', st0') ->
+                  (Forall (wc_equation G (vars++st_clocks st0')) eqs' /\
+                   wc_env (vars++st_clocks st0'))) a ->
+      (Forall (wc_equation G (vars++st_clocks st')) (concat eqs') /\
+       wc_env (vars++st_clocks st')).
+  Proof with eauto.
     intros G vars k a.
-    induction a; intros a1s eqs' st st' Hmap Hfollows Hforall;
-      simpl in Hmap; repeat inv_bind.
-    - constructor.
-    - apply Forall_app. split; eauto.
-      + rewrite Forall_forall in Hforall.
-        eapply Hforall; eauto.
-        * constructor. reflexivity.
-        * reflexivity.
-        * eapply map_bind2_st_follows in H0; eauto.
-          rewrite Forall_forall; intros; eauto.
-      + eapply IHa; eauto.
-        rewrite Forall_forall in *; intros.
-        eapply Hforall; eauto. apply in_cons; auto.
-        etransitivity; eauto.
+    induction a; intros a1s eqs' st st' Hwenv Hmap Hfollows Hforall;
+      repeat inv_bind; simpl in *...
+    assert (st_follows st x1) as Hfollows1 by eauto.
+    assert (st_follows x1 st') as Hfollows2 by repeat solve_st_follows.
+    rewrite Forall_forall in Hforall.
+    eapply Hforall in H as [Hwc' Hwenv']...
+    3,4:repeat solve_st_follows. 2:left...
+    eapply IHa in H0 as [Hwc'' Hwenv'']...
+    - split...
+      apply Forall_app. split...
+      solve_forall. repeat solve_incl.
+    - rewrite Forall_forall in *; intros.
+      eapply Hforall in H4... apply in_cons...
+      etransitivity...
   Qed.
 
   Fact add_whens_clockof : forall e ty ck,
@@ -879,36 +1064,64 @@ Module Type NCLOCKING
       + rewrite app_nil_r, add_whens_clockof...
       + apply fresh_ident_In in Hfresh.
         apply in_or_app; right.
-        unfold clock_of_nclock, stripname, st_clocks; simpl.
-        apply in_map_iff. exists (id, (Op.bool_type, cl, true))...
+        In_st_clocks id Op.bool_type cl true.
+  Qed.
+
+  Fact normalized_lexp_wc_exp_clockof : forall G vars e,
+      normalized_lexp e ->
+      wc_env vars ->
+      wc_exp G vars e ->
+      Forall (wc_clock vars) (clockof e).
+  Proof with eauto.
+    intros G vars e Hnormed Hwenv Hwc.
+    induction Hnormed; inv Hwc;
+      simpl; unfold clock_of_nclock, stripname; simpl; repeat constructor...
+    1,2:(unfold wc_env in Hwenv; rewrite Forall_forall in Hwenv; eapply Hwenv in H0; eauto).
+    - eapply IHHnormed in H1. rewrite H4 in H1. inv H1...
+    - eapply IHHnormed1 in H3. rewrite H6 in H3. inv H3...
+    - inv H3.
+      eapply IHHnormed in H1.
+      simpl in H7. rewrite app_nil_r in H7. symmetry in H7.
+      singleton_length.
+      inv H6. inv H1...
   Qed.
 
   Fact fby_iteexp_wc_eq : forall G vars e0 e a e' eqs' st st',
+      normalized_lexp e0 ->
+      wc_env (vars++st_clocks st) ->
       wc_exp G (vars++st_clocks st) e0 ->
       wc_exp G (vars++st_clocks st) e ->
-      clockof e = [(fst (snd a))] ->
       clockof e0 = [(fst (snd a))] ->
+      clockof e = [(fst (snd a))] ->
       unnamed_stream a ->
       fby_iteexp e0 e a st = (e', eqs', st') ->
       Forall (wc_equation G (vars++st_clocks st')) eqs'.
   Proof with eauto.
-    intros G vars e0 e [ty cl] e' eqs' st st' Hwc1 Hwc2 Hcl1 Hcl2 Hunnamed Hfby.
+    intros G vars e0 e [ty cl] e' eqs' st st' Hnormed Henv Hwc1 Hwc2 Hcl1 Hcl2 Hunnamed Hfby.
     unfold fby_iteexp in Hfby; simpl in *.
     destruct (Norm.is_constant e0); repeat inv_bind; repeat constructor; simpl...
-    - eapply add_whens_wc_exp... admit.
+    - eapply add_whens_wc_exp...
+      eapply normalized_lexp_wc_exp_clockof in Hnormed...
+      rewrite Hcl1 in Hnormed. inv Hnormed. repeat solve_incl.
     - repeat solve_incl.
     - rewrite app_nil_r, add_whens_clockof...
-    - rewrite app_nil_r. rewrite Hcl1...
+    - rewrite app_nil_r. rewrite Hcl2...
     - unfold unnamed_stream in Hunnamed; simpl in Hunnamed. rewrite Hunnamed. constructor.
     - eapply fresh_ident_In in H0.
-      apply in_or_app; right. unfold st_clocks.
-      apply in_map_iff. exists (x2, (ty, fst cl, false)); auto.
-    - eapply init_var_for_clock_wc_eq with (G:=G) (vars:=vars) in H...
-      2: admit.
-      solve_forall. repeat solve_incl.
-  Admitted.
+      apply in_or_app; right.
+      destruct cl. unfold clock_of_nclock, stripname; simpl in *.
+      In_st_clocks x2 ty c false.
+    - assert (st_follows st x1) as Hfollows1 by repeat solve_st_follows.
+      eapply init_var_for_clock_wc_eq with (G:=G) (vars:=(vars++st_clocks st)) in H...
+      2: { eapply normalized_lexp_wc_exp_clockof in Hnormed...
+           rewrite Hcl1 in Hnormed. inv Hnormed... }
+      solve_forall. solve_incl.
+      rewrite <- app_assoc. apply incl_appr', incl_app; repeat solve_incl.
+  Qed.
 
   Fact normalize_fby_wc_eq : forall G vars anns e0s es es' eqs' st st',
+      Forall normalized_lexp e0s ->
+      wc_env (vars++st_clocks st) ->
       Forall (wc_exp G (vars++st_clocks st)) e0s ->
       Forall (wc_exp G (vars++st_clocks st)) es ->
       Forall2 (fun e0 a => clockof e0 = [fst (snd a)]) e0s anns ->
@@ -917,10 +1130,10 @@ Module Type NCLOCKING
       normalize_fby e0s es anns st = (es', eqs', st') ->
       Forall (wc_equation G (vars++st_clocks st')) eqs'.
   Proof with eauto.
-    induction anns; intros e0s es es' eqs' st st' Hwc1 Hwc2 Hcl1 Hcl2 Hunnamed Hnorm;
+    induction anns; intros e0s es es' eqs' st st' Hnormed Hwenv Hwc1 Hwc2 Hcl1 Hcl2 Hunnamed Hnorm;
       inv Hcl1; inv Hcl2;
         unfold normalize_fby in Hnorm; simpl in Hnorm; repeat inv_bind; simpl...
-    inv Hwc1; inv Hwc2; inv Hunnamed.
+    inv Hnormed; inv Hwc1; inv Hwc2; inv Hunnamed.
     apply Forall_app; split.
     - clear IHanns.
       eapply fby_iteexp_wc_eq in H...
@@ -928,6 +1141,9 @@ Module Type NCLOCKING
     - assert (normalize_fby l l0 anns x4 = (x5, concat x6, st')) as Hnorm.
       { unfold normalize_fby; repeat inv_bind. repeat eexists... inv_bind... }
       eapply IHanns in Hnorm...
+      + destruct a as [ty cl]. eapply fby_iteexp_wc_env in H...
+        eapply normalized_lexp_wc_exp_clockof in H9...
+        rewrite H2 in H9. inv H9...
       + solve_forall. repeat solve_incl.
       + solve_forall. repeat solve_incl.
   Qed.
@@ -942,48 +1158,68 @@ Module Type NCLOCKING
     inv Hnormed; simpl in *; try destruct cl; repeat inv_bind; repeat constructor; simpl in *.
     2,5,8: repeat solve_incl.
     2,4,6:inv Hwc; simpl; auto.
-    1,2,3,4:eapply in_or_app; right; unfold st_clocks; rewrite in_map_iff.
-    - apply fresh_ident_In in H. exists (x, (Op.type_const c, Cbase, false))...
-    - apply fresh_ident_In in H0. exists (x, (ty, c, false))...
-    - apply fresh_ident_In in H1. exists (x, (ty, c, false))...
-    - apply fresh_ident_In in H0. exists (x0, (ty, c, false))...
+    1,2,3,4:eapply in_or_app; right.
+    1:apply fresh_ident_In in H; In_st_clocks x (Op.type_const c) Cbase false.
+    1,3:apply fresh_ident_In in H0. 3:apply fresh_ident_In in H1.
+    1,3:In_st_clocks x ty c false.
+    In_st_clocks x0 ty c false.
   Qed.
 
   Fact normalize_exp_wc_eq : forall G vars e is_control es' eqs' st st',
+      wc_global G ->
+      wc_env (vars++st_clocks st) ->
       wc_exp G (vars++st_clocks st) e ->
       normalize_exp is_control e st = (es', eqs', st') ->
-      Forall (wc_equation G (vars++st_clocks st')) eqs'.
+      Forall (wc_equation G (vars++st_clocks st')) eqs' /\
+      wc_env (vars++st_clocks st').
   Proof with eauto.
-    induction e using exp_ind2; intros is_control es' eqs' st st' Hwc Hnorm;
-      simpl in *; inv Hwc; repeat inv_bind...
+    induction e using exp_ind2; intros is_control es' eqs' st st' HwG Hwenv Hwc Hnorm;
+      assert (Hnorm':=Hnorm); apply normalize_exp_fresh_incl in Hnorm';
+      simpl in *;
+      assert (Hwc':=Hwc); inv Hwc'; repeat inv_bind...
     - (* binop *)
-      assert (st_follows st x1) as Hfollows by eauto. eapply st_follows_clocks_incl in Hfollows.
+      assert (st_follows st x1) as Hfollows by eauto.
+      eapply IHe1 in H as [Hwc1 Hwenv1]...
       assert (st_follows x1 st') as Hfollows2 by eauto.
-      eapply IHe1 in H...
-      eapply IHe2 in H0... 2: repeat solve_incl.
-      eapply Forall_app; split...
+      eapply IHe2 in H0 as [Hwc2 Hwenv2]... 2: repeat solve_incl.
+      split... eapply Forall_app; split...
       solve_forall. repeat solve_incl.
     - (* fby *)
+      assert (st_follows st x1) as Hfollows1 by repeat solve_st_follows.
+      assert (st_follows x1 x4) as Hfollows2 by repeat solve_st_follows.
+      assert (st_follows x4 x7) as Hfollows3 by repeat solve_st_follows.
+      assert (st_follows x7 st') as Hfollows4 by repeat solve_st_follows.
       rewrite Forall2_eq in H6, H7.
       assert (length (concat x2) = length (annots e0s)) as Hlen1 by eauto.
       assert (length (concat x9) = length (annots es)) as Hlen2 by eauto.
-      assert (length x5 = length a) as Hlen3.
+      assert (length a = length x5) as Hlen4.
       { repeat simpl_length.
         eapply normalize_fby_length in H3...
         1,2:symmetry;erewrite <- map_length.
         + setoid_rewrite H6; solve_length.
         + setoid_rewrite H7; solve_length. }
-      repeat rewrite Forall_app; repeat split.
+      assert (length x8 = length x5) as Hlen3.
+      { eapply idents_for_anns_length in H9. solve_length. }
+      specialize (normalize_fby_numstreams _ _ _ _ _ _ _ H3) as Hnumstreams.
+      assert (H1':=H1).
+      eapply map_bind2_wc_eq in H1' as [Hwc1 Hwenv1]...
+      2: { rewrite Forall_forall in *; intros; simpl in *.
+           eapply H... eapply H4 in H10. repeat solve_incl. }
+      assert (H2':=H2).
+      eapply map_bind2_wc_eq in H2' as [Hwc2 Hwenv2]...
+      2: { rewrite Forall_forall in *; intros; simpl in *.
+           eapply H0... eapply H5 in H10. repeat solve_incl. }
+      clear H H0.
+      split; repeat rewrite Forall_app; repeat split.
       + assert (st_follows x4 st') as Hfollows by repeat solve_st_follows.
         assert (annots x5 = a) as Hanns.
         { repeat simpl_length.
           eapply normalize_fby_annot in H3...
           + erewrite Hlen1, <- map_length, <- map_length. setoid_rewrite <- H6. apply map_length.
           + erewrite Hlen2, <- map_length, <- map_length. setoid_rewrite <- H7. apply map_length. } subst.
-        eapply normalize_fby_wc_exp' in H3.
-        3,4:unfold normalize_exps; repeat inv_bind; repeat eexists; repeat inv_bind; try reflexivity; eauto.
-        2: eauto.
-        clear H H0 H4 H5 H6 H7.
+        eapply normalize_fby_wc_exp' in H3...
+        2,3:unfold normalize_exps; repeat inv_bind; repeat eexists; repeat inv_bind; try reflexivity; eauto.
+        clear H4 H5 H6 H7.
         rewrite Forall_map.
         repeat rewrite_Forall_forall.
         destruct x as [[x ann] e]; repeat constructor.
@@ -991,173 +1227,264 @@ Module Type NCLOCKING
           solve_incl. rewrite <- app_assoc.
           apply incl_appr', incl_app; solve_incl.
         * apply idents_for_anns_values in H9.
-          repeat simpl_nth. 2:erewrite <- map_length, H9; auto.
+          repeat simpl_nth.
+          assert (In e x5) as Hin. { repeat simpl_length. eapply nth_In in H. rewrite H6 in H... }
           simpl; rewrite app_nil_r, H6.
-          admit. (* ok because we know unnamed_stream *)
-        * admit. (* idem *)
-      + eapply map_bind2_wc_eq in H1...
-        rewrite Forall_forall in H, H4. rewrite Forall_forall; intros.
-        eapply H in H10; [| |eauto].
-        solve_forall; repeat solve_incl.
-        eapply H4 in H10. repeat solve_incl.
-      + eapply map_bind2_wc_eq in H2...
-        rewrite Forall_forall in H0, H5. rewrite Forall_forall; intros.
-        eapply H0 in H10; [| |eauto].
-        solve_forall; repeat solve_incl.
-        eapply H5 in H10; repeat solve_incl.
-      + admit. (* The equations generated by normalize_fby should be wc *)
+          assert (Forall unnamed_stream (annot e)).
+          { rewrite Forall_forall. intros ann' Hin'.
+            apply H8. unfold annots; rewrite flat_map_concat_map.
+            eapply in_concat'... apply in_map... }
+          apply Hnumstreams in Hin.
+          rewrite nclockof_annot. rewrite <- length_annot_numstreams in Hin. singleton_length.
+          repeat constructor. inv H0. inv H10. rewrite H4. constructor.
+        * assert (numstreams e = 1).
+          { eapply Hnumstreams. repeat simpl_In... }
+          rewrite <- length_clockof_numstreams in H0. singleton_length.
+          assert ([c] = map (fun x => (fst (snd x))) [ann]); subst.
+          { repeat simpl_nth. apply idents_for_anns_values in H9.
+            rewrite split_nth in H5; inv H5.
+            rewrite split_map_snd, H9.
+            unfold annots. erewrite flat_map_concat_map, <- concat_length_map_nth.
+            2: solve_length. 2:{ rewrite Forall_forall; intros. rewrite length_annot_numstreams... }
+            rewrite H6. rewrite clockof_annot, map_map in Hsingl... }
+          simpl in H0. inv H0.
+          repeat constructor. apply in_or_app; right.
+          apply idents_for_anns_incl_clocks in H9. apply H9.
+          repeat simpl_In. exists (x, ann).
+          destruct ann as [? [? ?]]...
+      + solve_forall. repeat solve_incl.
+      + solve_forall. repeat solve_incl.
+      + eapply normalize_fby_wc_eq with (G:=G) (vars:=vars) in H3...
+        * solve_forall. repeat solve_incl.
+        * eapply map_bind2_normalize_exp_wc_exp with (G:=G) (vars:=vars) in H1...
+          1,2:solve_forall; repeat solve_incl.
+        * eapply map_bind2_normalize_exp_wc_exp with (G:=G) (vars:=vars) in H2...
+          1,2:solve_forall; repeat solve_incl.
+        * assert (H1':=H1). eapply map_bind2_normalize_exp_numstreams in H1'.
+          eapply map_bind2_normalize_exp_clocksof' in H1...
+          assert (Forall2 (fun e a => clockof e = [a]) (concat x2) (map clock_of_nclock a)).
+          { rewrite H6. unfold clocksof. rewrite flat_map_concat_map.
+            apply Forall2_concat. rewrite Forall2_map_2.
+            eapply Forall2_impl_In... intros; simpl in *. rewrite <- H10.
+            unfold clocksof. rewrite flat_map_concat_map. rewrite <- (concat_map_singl1 a0) at 1.
+            apply Forall2_concat. rewrite Forall2_map_2, Forall2_map_1, <- Forall2_same.
+            apply Forall_forall. intros ? Hin.
+            assert (length (clockof x) = 1).
+            { rewrite length_clockof_numstreams. rewrite Forall_forall in H1'; apply H1'. eapply in_concat'... }
+            singleton_length. repeat constructor...
+          }
+          rewrite Forall2_map_2 in H...
+        * assert (H2':=H2). eapply map_bind2_normalize_exp_numstreams in H2'.
+          eapply map_bind2_normalize_exp_clocksof' in H2...
+          assert (Forall2 (fun e a => clockof e = [a]) (concat x9) (map clock_of_nclock a)).
+          { rewrite H7. unfold clocksof. rewrite flat_map_concat_map.
+            apply Forall2_concat. rewrite Forall2_map_2.
+            eapply Forall2_impl_In... intros; simpl in *. rewrite <- H10.
+            unfold clocksof. rewrite flat_map_concat_map. rewrite <- (concat_map_singl1 a0) at 1.
+            apply Forall2_concat. rewrite Forall2_map_2, Forall2_map_1, <- Forall2_same.
+            apply Forall_forall. intros ? Hin.
+            assert (length (clockof x) = 1).
+            { rewrite length_clockof_numstreams. rewrite Forall_forall in H2'; apply H2'. eapply in_concat'... }
+            singleton_length. repeat constructor...
+          }
+          rewrite Forall2_map_2 in H...
+      + assert (Forall (wc_clock ((vars ++ st_clocks x1))) (map clock_of_nclock a)).
+        { rewrite H6.
+          eapply wc_exp_clocksof in H4... eapply Forall_impl; [|eauto]. intros.
+          eapply wc_clock_incl; [|eauto]. rewrite <- app_assoc in *.
+          apply incl_appr', incl_app; repeat solve_incl.
+          apply map_bind2_normalize_exp_fresh_incl in H1...
+          unfold st_clocks. apply incl_map, H1. }
+        eapply normalize_fby_wc_env in H3...
+        2:{ rewrite Forall_map in H. eapply Forall_impl...
+            intros [ty [cl name]] Hwc'.
+            unfold clock_of_nclock, stripname in Hwc'; simpl in Hwc'.
+            repeat solve_incl. }
+      eapply idents_for_anns_wc_env in H9...
+      unfold clock_of_nclock, stripname in H. rewrite map_map.
+      eapply Forall_impl; [|eauto]. intros.
+      repeat solve_incl.
     - (* when *)
-      eapply map_bind2_wc_eq in H0...
+      eapply map_bind2_wc_eq in H0 as [Hwc1 Hwenv1]...
       rewrite Forall_forall in H, H4. rewrite Forall_forall; intros.
-      eapply H in H1; [| |eauto].
-      solve_forall; repeat solve_incl.
+      eapply H in H1. 1,2,3,5:eauto.
       apply H4 in H1; repeat solve_incl.
     - (* merge *)
       assert (length (concat x3) = length (annots ets)) as Hlen1 by eauto.
       assert (length (concat x6) = length (annots efs)) as Hlen2 by eauto.
+      assert (H1':=H1).
+      eapply map_bind2_wc_eq in H1' as [Hwc1 Hwenv1]...
+      2: { rewrite Forall_forall in *; intros; simpl in *.
+           eapply H... eapply H5 in H4. repeat solve_incl. }
+      assert (H2':=H2).
+      eapply map_bind2_wc_eq in H2' as [Hwc2 Hwenv2]...
+      2: { rewrite Forall_forall in *; intros; simpl in *.
+           eapply H0... eapply H6 in H4. repeat solve_incl. }
+      clear H H0.
       destruct is_control; repeat inv_bind; repeat rewrite Forall_app; repeat split.
-      1,4: eapply map_bind2_wc_eq in H1... 3,5: eapply map_bind2_wc_eq in H2...
-      1,2,3,4: repeat rewrite_Forall_forall.
-      Local Ltac mergeiteeqs Hin1 Hin2 Hind Hnorm Hwc :=
-        eapply Hind in Hnorm; eauto;
-        [rewrite Forall_forall in Hnorm; eapply Hnorm in Hin2; repeat solve_incl
-        |eapply Hwc in Hin1; repeat solve_incl].
-      + mergeiteeqs H3 H14 H H4 H5.
-      + mergeiteeqs H4 H15 H H12 H5.
-      + mergeiteeqs H3 H14 H0 H4 H6.
-      + mergeiteeqs H4 H15 H0 H12 H6.
-      + clear H H0.
-        assert (length x0 = length tys) as Hlen3 by (eapply idents_for_anns_length in H3; solve_length).
-        apply Forall2_combine'.
-        rewrite Forall2_map_1, map_map, Forall2_map_2.
-        repeat rewrite_Forall_forall...
-        * solve_length.
-        * destruct nth as [[? ?] ?] eqn:Hnth. inv H0; [|inv H4].
-          destruct b as [[? ?] ?]; repeat simpl_nth.
-          repeat constructor; simpl; try rewrite app_nil_r.
-          Local Ltac mergeitelength H :=
-            rewrite length_clockof_numstreams; symmetry;
-            apply map_bind2_normalize_exp_numstreams in H; rewrite Forall_forall in H;
-            apply H, nth_In; solve_length.
-          -- eapply map_bind2_normalize_exp_wc_exp with (vars:=vars) in H1...
-             1,2:rewrite Forall_forall in *; intros.
-             eapply wc_exp_incl; [| eapply H1, nth_In; solve_length]. repeat solve_incl.
-             eapply wc_exp_incl; [| eauto]. repeat solve_incl.
-          -- eapply map_bind2_normalize_exp_wc_exp with (vars:=vars) in H2...
-             1,2:rewrite Forall_forall in *; intros.
-             eapply wc_exp_incl; [| eapply H2, nth_In; solve_length]. repeat solve_incl.
-             eapply wc_exp_incl; [| eauto]. repeat solve_incl.
-          -- assert (incl (vars++st_clocks st) (vars++st_clocks st')) by repeat solve_incl.
-             rewrite <- H4; eauto.
-          -- rewrite Forall_forall; intros.
-             eapply H8. erewrite <- map_bind2_normalize_exp_clocksof... 2:rewrite Forall_forall...
-             unfold clocksof; rewrite flat_map_concat_map.
-             eapply concat_map_incl... eapply nth_In; solve_length.
-          -- rewrite Forall_forall; intros.
-             eapply H9. erewrite <- map_bind2_normalize_exp_clocksof... 2:rewrite Forall_forall...
-             unfold clocksof; rewrite flat_map_concat_map.
-             eapply concat_map_incl... eapply nth_In; solve_length.
-          -- mergeitelength H1.
-          -- mergeitelength H2.
-        * destruct nth, nth, p...
-        * destruct nth; simpl in H0. destruct n0; try omega; simpl.
-          destruct (nth n _ _) as [[? ?] ?]; simpl...
-        * destruct nth, nth, p...
-        * destruct nth as [? [? [? ?]]] eqn:Hi; simpl in H0. destruct n0; try omega; simpl.
-          destruct (nth n (combine _ _) _) as [[? ?] ?] eqn:Hi2; simpl...
-          unfold clock_of_nclock, stripname; simpl.
-          assert (c = ck); subst. {
-            apply idents_for_anns_values in H3.
-            specialize (map_nth snd x0 a n) as Hmap.
-            rewrite H3, Hi, map_nth' with (d':=Op.bool_type) in Hmap; simpl in Hmap; inv Hmap; auto.
-            solve_length. }
-          apply idents_for_anns_incl_clocks in H3.
-          apply in_or_app. right. apply H3.
-          rewrite in_map_iff. exists (i, (t, (ck, o))); split...
-          setoid_rewrite <- Hi...
+      1,2,5,6:(solve_forall; repeat solve_incl). 1:eauto.
+      2:{ eapply idents_for_anns_wc_env in H...
+          repeat rewrite Forall_map.
+          rewrite Forall_forall. intros ty _; simpl.
+          unfold wc_env in Hwenv; rewrite Forall_forall in Hwenv; eapply Hwenv in H7; simpl in H7.
+          repeat solve_incl. }
+      apply Forall2_combine'.
+      assert (length x0 = length tys) as Hlen3 by (eapply idents_for_anns_length in H; solve_length).
+      rewrite Forall2_map_1, map_map, Forall2_map_2.
+      repeat rewrite_Forall_forall...
+      + solve_length.
+      + destruct nth as [[? ?] ?] eqn:Hnth. inv H3; [|inv H4].
+        destruct b as [[? ?] ?]; repeat simpl_nth.
+        repeat constructor; simpl; try rewrite app_nil_r.
+        Local Ltac mergeitelength H :=
+          rewrite length_clockof_numstreams; symmetry;
+          apply map_bind2_normalize_exp_numstreams in H; rewrite Forall_forall in H;
+          apply H, nth_In; solve_length.
+        * eapply map_bind2_normalize_exp_wc_exp with (vars:=vars) in H1...
+           1,2:rewrite Forall_forall in *; intros...
+           eapply wc_exp_incl; [| eapply H1, nth_In; solve_length]. repeat solve_incl.
+        * eapply map_bind2_normalize_exp_wc_exp with (vars:=vars) in H2...
+           1,2:rewrite Forall_forall in *; intros...
+           eapply wc_exp_incl; [| eapply H2, nth_In; solve_length]. repeat solve_incl.
+           eapply wc_exp_incl; [| eauto]. repeat solve_incl.
+        * assert (incl (vars++st_clocks st) (vars++st_clocks st')) by repeat solve_incl.
+           rewrite <- H4; eauto.
+        * rewrite Forall_forall; intros.
+           eapply H8. erewrite <- map_bind2_normalize_exp_clocksof... 2:rewrite Forall_forall...
+           unfold clocksof; rewrite flat_map_concat_map.
+           eapply concat_map_incl... eapply nth_In; solve_length.
+        * rewrite Forall_forall; intros.
+           eapply H9. erewrite <- map_bind2_normalize_exp_clocksof... 2:rewrite Forall_forall...
+           unfold clocksof; rewrite flat_map_concat_map.
+           eapply concat_map_incl... eapply nth_In; solve_length.
+        * mergeitelength H1.
+        * mergeitelength H2.
+      + destruct nth, nth, p...
+      + destruct nth; simpl in H3. destruct n0; try omega; simpl.
+        destruct (nth n _ _) as [[? ?] ?]; simpl...
+      + destruct nth, nth, p...
+      + destruct nth as [? [? [? ?]]] eqn:Hi; simpl in H3. destruct n0; try omega; simpl.
+        destruct (nth n (combine _ _) _) as [[? ?] ?] eqn:Hi2; simpl...
+        unfold clock_of_nclock, stripname; simpl.
+        assert (c = ck); subst. {
+          apply idents_for_anns_values in H.
+          specialize (map_nth snd x0 a n) as Hmap.
+          rewrite H, Hi, map_nth' with (d':=Op.bool_type) in Hmap; simpl in Hmap; inv Hmap; auto.
+          solve_length. }
+        apply idents_for_anns_incl_clocks in H.
+        apply in_or_app. right. apply H.
+        rewrite in_map_iff. exists (i, (t, (ck, o))); split...
+        setoid_rewrite <- Hi...
     - (* ite *)
       assert (length (concat x5) = length (annots ets)) as Hlen1 by eauto.
       assert (length (concat x8) = length (annots efs)) as Hlen2 by eauto.
+      assert (H1':=H1).
+      eapply IHe in H1' as [Hwc1 Hwenv1]...
+      assert (H2':=H2).
+      eapply map_bind2_wc_eq in H2' as [Hwc2 Hwenv2]...
+      2: { rewrite Forall_forall in *; intros; simpl in *.
+           eapply H... eapply H6 in H14. repeat solve_incl. }
+      assert (H3':=H3).
+      eapply map_bind2_wc_eq in H3' as [Hwc3 Hwenv3]...
+      2: { rewrite Forall_forall in *; intros; simpl in *.
+           eapply H0... eapply H7 in H14. repeat solve_incl. }
+      clear H H0 IHe.
       destruct is_control; repeat inv_bind; repeat rewrite Forall_app; repeat split.
-      2,6: eapply map_bind2_wc_eq in H2... 4,7: eapply map_bind2_wc_eq in H3...
-      1,7:eapply IHe in H1; eauto; solve_forall; repeat solve_incl.
-      1,2,3,4: repeat rewrite_Forall_forall.
-      + mergeiteeqs H4 H17 H H14 H6.
-      + mergeiteeqs H14 H18 H H15 H6.
-      + mergeiteeqs H4 H17 H0 H14 H7.
-      + mergeiteeqs H14 H18 H0 H15 H7.
-      + clear H H0.
-        assert (length x2 = length tys) as Hlen3 by (eapply idents_for_anns_length in H4; solve_length).
+      1,2,3,6,7,8:solve_forall;repeat solve_incl. 1:eauto.
+      2:{ eapply idents_for_anns_wc_env in H...
+          repeat rewrite Forall_map.
+          rewrite Forall_forall. intros ty _; simpl.
+          eapply wc_exp_clockof in H5... rewrite H8 in H5. inv H5.
+          solve_incl. rewrite <- app_assoc. apply incl_appr', incl_app; [repeat solve_incl|].
+          unfold st_clocks. apply incl_map.
+          eapply normalize_exp_fresh_incl in H1. etransitivity...
+          apply incl_map, st_follows_incl. repeat solve_st_follows. }
+        assert (length x2 = length tys) as Hlen3 by (eapply idents_for_anns_length in H; solve_length).
         apply Forall2_combine'.
         rewrite Forall2_map_1, map_map, Forall2_map_2.
         repeat rewrite_Forall_forall...
-        * solve_length.
-        * destruct nth as [[? ?] ?] eqn:Hnth. inv H0; [|inv H4].
+        + solve_length.
+        + destruct nth as [[? ?] ?] eqn:Hnth. inv H4; [|inv H14].
           destruct b as [[? ?] ?]; repeat simpl_nth.
           repeat constructor; simpl; try rewrite app_nil_r.
-          -- eapply hd_default_wc_exp. eapply normalize_exp_wc_exp in H1...
-             solve_forall. repeat solve_incl.
-          -- eapply map_bind2_normalize_exp_wc_exp with (vars:=vars) in H2...
-             1,2:rewrite Forall_forall in *; intros.
-             eapply wc_exp_incl; [| eapply H2, nth_In; solve_length]. repeat solve_incl.
-             eapply wc_exp_incl; [| eauto]. repeat solve_incl.
-          -- eapply map_bind2_normalize_exp_wc_exp with (vars:=vars) in H3...
-             1,2:rewrite Forall_forall in *; intros.
-             eapply wc_exp_incl; [| eapply H3, nth_In; solve_length]. repeat solve_incl.
-             eapply wc_exp_incl; [| eauto]. repeat solve_incl.
-          -- assert (length x = numstreams e) as Hlen4 by eauto.
-             rewrite <- length_clockof_numstreams, H8 in Hlen4; simpl in Hlen4.
-             erewrite <- normalize_exp_clockof in H8...
-             repeat singleton_length...
-          -- rewrite Forall_forall; intros.
-             eapply H9. erewrite <- map_bind2_normalize_exp_clocksof... 2:rewrite Forall_forall...
-             unfold clocksof; rewrite flat_map_concat_map.
-             eapply concat_map_incl... eapply nth_In; solve_length.
-          -- rewrite Forall_forall; intros.
-             eapply H10. erewrite <- map_bind2_normalize_exp_clocksof... 2:rewrite Forall_forall...
-             unfold clocksof; rewrite flat_map_concat_map.
-             eapply concat_map_incl... eapply nth_In; solve_length.
-          -- mergeitelength H2.
-          -- mergeitelength H3.
-          -- inv H14.
-        * destruct nth, nth, p...
-        * destruct nth; simpl in H0. destruct n0; try omega; simpl.
+          * eapply hd_default_wc_exp. eapply normalize_exp_wc_exp in H1...
+            solve_forall. repeat solve_incl.
+          * eapply map_bind2_normalize_exp_wc_exp with (vars:=vars) in H2...
+            1,2:rewrite Forall_forall in *; intros.
+            eapply wc_exp_incl; [| eapply H2, nth_In; solve_length]. repeat solve_incl.
+            eapply wc_exp_incl; [| eauto]. repeat solve_incl.
+          * eapply map_bind2_normalize_exp_wc_exp with (vars:=vars) in H3...
+            1,2:rewrite Forall_forall in *; intros.
+            eapply wc_exp_incl; [| eapply H3, nth_In; solve_length]. repeat solve_incl.
+            eapply wc_exp_incl; [| eauto]. repeat solve_incl.
+          * assert (length x = numstreams e) as Hlen4 by eauto.
+            rewrite <- length_clockof_numstreams, H8 in Hlen4; simpl in Hlen4.
+            erewrite <- normalize_exp_clockof in H8...
+            repeat singleton_length...
+          * rewrite Forall_forall; intros.
+            eapply H9. erewrite <- map_bind2_normalize_exp_clocksof... 2:rewrite Forall_forall...
+            unfold clocksof; rewrite flat_map_concat_map.
+            eapply concat_map_incl... eapply nth_In; solve_length.
+          * rewrite Forall_forall; intros.
+            eapply H10. erewrite <- map_bind2_normalize_exp_clocksof... 2:rewrite Forall_forall...
+            unfold clocksof; rewrite flat_map_concat_map.
+            eapply concat_map_incl... eapply nth_In; solve_length.
+          * mergeitelength H2.
+          * mergeitelength H3.
+        + destruct nth, nth, p...
+        + destruct nth; simpl in H4. destruct n0; try omega; simpl.
           destruct (nth n _ _) as [[? ?] ?]; simpl...
-        * destruct nth, nth, p...
-        * destruct nth as [? [? [? ?]]] eqn:Hi; simpl in H0. destruct n0; try omega; simpl.
+        + destruct nth, nth, p...
+        + destruct nth as [? [? [? ?]]] eqn:Hi; simpl in H4. destruct n0; try omega; simpl.
           destruct (nth n (combine _ _) _) as [[? ?] ?] eqn:Hi2; simpl...
           unfold clock_of_nclock, stripname; simpl.
           assert (c = ck); subst. {
-            apply idents_for_anns_values in H4.
+            apply idents_for_anns_values in H.
             specialize (map_nth snd x2 a n) as Hmap.
-            rewrite H4, Hi, map_nth' with (d':=Op.bool_type) in Hmap; simpl in Hmap; inv Hmap; auto.
+            rewrite H, Hi, map_nth' with (d':=Op.bool_type) in Hmap; simpl in Hmap; inv Hmap; auto.
             solve_length. }
-          apply idents_for_anns_incl_clocks in H4.
-          apply in_or_app. right. apply H4.
+          apply idents_for_anns_incl_clocks in H.
+          apply in_or_app. right. apply H.
           rewrite in_map_iff. exists (i, (t, (ck, o))); split...
           setoid_rewrite <- Hi...
     - (* app *)
-      rewrite app_nil_r. constructor.
+      rewrite app_nil_r.
+      assert (H1':=H1).
+      eapply map_bind2_wc_eq in H1' as [Hwc1 Hwenv1]...
+      2:{ rewrite Forall_forall in *; intros. eapply H0...
+          eapply H5 in H3. repeat solve_incl. } clear H0.
+      repeat constructor; simpl...
       + repeat econstructor; simpl...
         * eapply map_bind2_normalize_exp_wc_exp in H1...
           solve_forall. repeat solve_incl.
         * erewrite map_bind2_normalize_exp_nclocksof...
         * erewrite idents_for_anns'_values...
-        * rewrite app_nil_r, map_map, Forall2_map_1, Forall2_map_2, <- Forall2_same.
-          eapply idents_for_anns'_clocknames...
-        * unfold clock_of_nclock, stripname.
-          rewrite app_nil_r, map_map, Forall2_map_1, Forall2_map_2, <- Forall2_same.
-          eapply idents_for_anns'_incl_clocks in H2.
-          apply Forall_forall; intros.
-          apply in_or_app; right. apply H2.
-          rewrite in_map_iff. exists x; split; auto. destruct x as [? [? [? ?]]]; auto.
-      + eapply map_bind2_wc_eq in H1...
-        rewrite Forall_forall in *. intros.
-        eapply H0 in H4... solve_forall; repeat solve_incl.
-        eapply H5 in H3. repeat solve_incl.
+      + rewrite app_nil_r, map_map, Forall2_map_1, Forall2_map_2, <- Forall2_same.
+        eapply idents_for_anns'_clocknames...
+      + unfold clock_of_nclock, stripname.
+        rewrite app_nil_r, map_map, Forall2_map_1, Forall2_map_2, <- Forall2_same.
+        eapply idents_for_anns'_incl_clocks in H2.
+        apply Forall_forall; intros.
+        apply in_or_app; right. apply H2.
+        rewrite in_map_iff. exists x; split; auto. destruct x as [? [? [? ?]]]; auto.
+      + solve_forall. repeat solve_incl.
+      + eapply idents_for_anns'_wc_env...
+        apply wc_exp_clockof in Hwc...
+        unfold clock_of_nclock, stripname in Hwc.
+        rewrite map_map. eapply Forall_impl; [|eauto].
+        intros. rewrite <- app_assoc in H0. repeat solve_incl.
+        apply incl_app; [repeat solve_incl|].
+        unfold st_clocks. apply incl_map...
     - (* app (reset) *)
+      assert (H1':=H1).
+      eapply map_bind2_wc_eq in H1' as [Hwc1 Hwenv1]...
+      2:{ rewrite Forall_forall in *; intros. eapply H0...
+          eapply H5 in H11. repeat solve_incl. }
+      assert (H2':=H2).
+      eapply H in H2' as [Hwc2 Hwenv2]... 2:repeat solve_incl.
+      clear H H0.
       rewrite cons_is_app.
-      repeat rewrite Forall_app. repeat split.
+      repeat constructor; repeat rewrite Forall_app; repeat split; simpl...
       + repeat econstructor; simpl...
         * eapply map_bind2_normalize_exp_wc_exp in H1...
           solve_forall. repeat solve_incl.
@@ -1173,64 +1500,128 @@ Module Type NCLOCKING
           eapply normalize_exp_clockof in H2... simpl in H2; rewrite app_nil_r, H10 in H2; clear H10.
           assert (numstreams e = 1) as Hnum by (rewrite <- length_clockof_numstreams, H2; eauto).
           eapply normalize_reset_clockof in Hnum... rewrite Hnum, H2...
-        * rewrite app_nil_r, map_map, Forall2_map_1, Forall2_map_2, <- Forall2_same.
-          eapply idents_for_anns'_clocknames...
-        * unfold clock_of_nclock, stripname.
-          rewrite app_nil_r, map_map, Forall2_map_1, Forall2_map_2, <- Forall2_same.
-          eapply idents_for_anns'_incl_clocks in H3.
-          apply Forall_forall; intros.
-          apply in_or_app; right. apply H3.
-          rewrite in_map_iff. exists x; split; auto. destruct x as [? [? [? ?]]]; auto.
-      + eapply map_bind2_wc_eq in H1...
-        rewrite Forall_forall in *. intros.
-        eapply H0 in H12... solve_forall; repeat solve_incl.
-        eapply H5 in H11. repeat solve_incl.
-      + eapply H in H2... solve_forall; repeat solve_incl.
-        repeat solve_incl.
+      + rewrite app_nil_r, map_map, Forall2_map_1, Forall2_map_2, <- Forall2_same.
+        eapply idents_for_anns'_clocknames...
+      + unfold clock_of_nclock, stripname.
+        rewrite app_nil_r, map_map, Forall2_map_1, Forall2_map_2, <- Forall2_same.
+        eapply idents_for_anns'_incl_clocks in H3.
+        apply Forall_forall; intros.
+        apply in_or_app; right. apply H3.
+        rewrite in_map_iff. exists x; split; auto. destruct x as [? [? [? ?]]]; auto.
+      + solve_forall; repeat solve_incl.
+      + solve_forall; repeat solve_incl.
       + eapply normalize_reset_wc_eq with (G:=G) (vars:=vars) in H4...
         solve_forall; repeat solve_incl.
         eapply hd_default_wc_exp.
         eapply normalize_exp_wc_exp in H2... repeat solve_incl.
-  Admitted.
+      + assert (length x6 = 1) as Hlen.
+        { eapply normalize_exp_length in H2... rewrite H2, <- length_clockof_numstreams, H10... }
+        singleton_length.
+        assert (clockof e = [ckr]) as Hck.
+        { eapply normalize_exp_clockof in H2... simpl in H2; rewrite app_nil_r in H2. congruence. }
+        specialize (normalize_exp_fresh_incl _ _ _ _ _ _ H2) as Hincl'.
+        assert (st_follows x8 st') as Hfollows3 by repeat solve_st_follows.
+        eapply normalize_reset_wc_env in H4...
+        2: { rewrite Hck. repeat constructor.
+             eapply wc_exp_clockof in H9...
+             rewrite H10 in H9; inv H9. rewrite <- app_assoc in H11.
+             repeat solve_incl. apply incl_app; [repeat solve_incl|].
+             unfold st_clocks. apply incl_map... }
+        eapply idents_for_anns'_wc_env in H3...
+        apply wc_exp_clockof in Hwc...
+        unfold clock_of_nclock, stripname in Hwc.
+        rewrite map_map. eapply Forall_impl; [|eauto].
+        intros. rewrite <- app_assoc in H. repeat solve_incl.
+        apply incl_app; [repeat solve_incl|].
+        unfold st_clocks. apply incl_map...
+  Qed.
 
   Corollary normalize_exps_wc_eq : forall G vars es es' eqs' st st',
+      wc_global G ->
+      wc_env (vars++st_clocks st) ->
       Forall (wc_exp G (vars++st_clocks st)) es ->
       normalize_exps es st = (es', eqs', st') ->
-      Forall (wc_equation G (vars++st_clocks st')) eqs'.
+      Forall (wc_equation G (vars++st_clocks st')) eqs' /\
+      wc_env (vars++st_clocks st').
   Proof with eauto.
-    intros G vars es es' eqs' st st' Hwc Hnorm.
+    intros G vars es es' eqs' st st' HwG Hwenv Hwc Hnorm.
     unfold normalize_exps in Hnorm; repeat inv_bind.
     eapply map_bind2_wc_eq in H...
     solve_forall.
-    eapply normalize_exp_wc_eq with (G:=G) (vars:=vars) in H1...
-    + solve_forall; repeat solve_incl.
-    + repeat solve_incl.
+    eapply normalize_exp_wc_eq with (G:=G) (vars:=vars) in H4...
+    repeat solve_incl.
   Qed.
 
   Fact normalize_rhs_wc_eq : forall G vars e keep_fby es' eqs' st st',
+      wc_global G ->
+      wc_env (vars++st_clocks st) ->
       wc_exp G (vars++st_clocks st) e ->
       normalize_rhs keep_fby e st = (es', eqs', st') ->
-      Forall (wc_equation G (vars++st_clocks st')) eqs'.
+      Forall (wc_equation G (vars++st_clocks st')) eqs' /\
+      wc_env (vars++st_clocks st').
   Proof with eauto.
-    intros G vars e keep_fby es' eqs' st st' Hwc Hnorm.
+    intros G vars e keep_fby es' eqs' st st' HwG Hwenv Hwc Hnorm.
     destruct e; unfold normalize_rhs in Hnorm;
       try (solve [eapply normalize_exp_wc_eq in Hnorm; eauto]);
       [destruct keep_fby|inv Hwc].
     - (* fby (keep) *)
-      inv Hwc.
+      assert (Hwc':=Hwc). inv Hwc'.
       repeat inv_bind.
-      repeat rewrite Forall_app; repeat split.
-      + eapply normalize_exps_wc_eq with (G:=G) (vars:=vars) in H...
-        solve_forall; repeat solve_incl.
-      + eapply normalize_exps_wc_eq with (G:=G) (vars:=vars) in H0...
-        1,2:solve_forall; repeat solve_incl.
+      assert (st_follows x1 x4) as Hfollows1 by repeat solve_st_follows.
+      assert (st_follows x4 st') as Hfollows2 by repeat solve_st_follows.
+      assert (H':=H).
+      eapply normalize_exps_wc_eq in H' as [Hwc1 Hwenv1]...
+      assert (H0':=H0).
+      eapply normalize_exps_wc_eq in H0' as [Hwc2 Hwenv2]...
+      2:solve_forall; repeat solve_incl.
+      split; repeat rewrite Forall_app; repeat split.
+      + solve_forall; repeat solve_incl.
+      + solve_forall; repeat solve_incl.
       + eapply normalize_fby_wc_eq in H1...
-        * eapply normalize_exps_wc_exp in H...
-          solve_forall; repeat solve_incl.
-        * eapply normalize_exps_wc_exp in H0...
-          solve_forall; repeat solve_incl.
-        * admit.
-        * admit.
+        * eapply normalize_exps_wc_exp in H... solve_forall. repeat solve_incl.
+        * eapply normalize_exps_wc_exp in H0... solve_forall. repeat solve_incl.
+        * unfold normalize_exps in H; repeat inv_bind.
+          assert (H':=H). eapply map_bind2_normalize_exp_numstreams in H'.
+          eapply map_bind2_normalize_exp_clocksof' in H...
+          assert (Forall2 (fun e a => clockof e = [a]) (concat x5) (map clock_of_nclock l1)).
+          { rewrite Forall2_eq in H4; rewrite H4. unfold clocksof. rewrite flat_map_concat_map.
+            apply Forall2_concat. rewrite Forall2_map_2.
+            eapply Forall2_impl_In... intros; simpl in *. rewrite <- H9.
+            unfold clocksof. rewrite flat_map_concat_map. rewrite <- (concat_map_singl1 a) at 1.
+            apply Forall2_concat. rewrite Forall2_map_2, Forall2_map_1, <- Forall2_same.
+            apply Forall_forall. intros ? Hin.
+            assert (length (clockof x) = 1).
+            { rewrite length_clockof_numstreams. rewrite Forall_forall in H'; apply H'. eapply in_concat'... }
+            singleton_length. repeat constructor...
+          }
+          rewrite Forall2_map_2 in H7...
+        * unfold normalize_exps in H0; repeat inv_bind.
+          assert (H0':=H0). eapply map_bind2_normalize_exp_numstreams in H0'.
+          eapply map_bind2_normalize_exp_clocksof' in H0...
+          assert (Forall2 (fun e a => clockof e = [a]) (concat x5) (map clock_of_nclock l1)).
+          { rewrite Forall2_eq in H5; rewrite H5. unfold clocksof. rewrite flat_map_concat_map.
+            apply Forall2_concat. rewrite Forall2_map_2.
+            eapply Forall2_impl_In... intros; simpl in *. rewrite <- H9.
+            unfold clocksof. rewrite flat_map_concat_map. rewrite <- (concat_map_singl1 a) at 1.
+            apply Forall2_concat. rewrite Forall2_map_2, Forall2_map_1, <- Forall2_same.
+            apply Forall_forall. intros ? Hin.
+            assert (length (clockof x2) = 1).
+            { rewrite length_clockof_numstreams. rewrite Forall_forall in H0'; apply H0'. eapply in_concat'... }
+            singleton_length. repeat constructor...
+          }
+          rewrite Forall2_map_2 in H7...
+      + eapply normalize_fby_wc_env in H1...
+        eapply wc_exp_clockof in Hwc...
+        simpl in Hwc.
+        rewrite Forall_map in Hwc. eapply Forall_impl; [|eapply Hwc].
+        intros [ty [cl name]] Hwc'.
+        unfold clock_of_nclock, stripname in Hwc'; simpl in Hwc'.
+        solve_incl. rewrite <- app_assoc.
+        repeat solve_incl. apply incl_app; try solve_incl.
+        apply incl_map, incl_app.
+        * eapply normalize_exps_fresh_incl in H...
+          etransitivity... apply incl_map, st_follows_incl...
+        * eapply normalize_exps_fresh_incl in H0...
     - (* fby (dont keep) *)
       eapply normalize_exp_wc_eq in Hnorm...
     - (* app *)
@@ -1238,16 +1629,152 @@ Module Type NCLOCKING
       eapply normalize_exps_wc_eq in H...
     - (* app (reset) *)
       repeat inv_bind.
+      assert (H':=H).
+      eapply normalize_exps_wc_eq in H' as [Hwc1 Hwenv1]...
+      assert (H0':=H0).
+      eapply normalize_exp_wc_eq with (G:=G) (vars:=vars) in H0' as [Hwc2 Hwenv2]...
       repeat rewrite Forall_app; repeat split.
-      + eapply normalize_exps_wc_eq in H...
-        solve_forall; repeat solve_incl.
-      + eapply normalize_exp_wc_eq with (G:=G) (vars:=vars) in H0...
-        * solve_forall. repeat solve_incl.
-        * repeat solve_incl.
+      + solve_forall; repeat solve_incl.
+      + solve_forall. repeat solve_incl.
       + eapply normalize_reset_wc_eq in H1...
         eapply hd_default_wc_exp. eapply normalize_exp_wc_exp in H0...
         repeat solve_incl.
-  Admitted.
+      + assert (length x4 = 1) as Hlen.
+        { eapply normalize_exp_length in H0... rewrite H0, <- length_clockof_numstreams, H8... }
+        singleton_length.
+        assert (clockof e = [ckr]) as Hck.
+        { eapply normalize_exp_clockof in H0... simpl in H0; rewrite app_nil_r in H0. congruence. }
+        specialize (normalize_exp_fresh_incl _ _ _ _ _ _ H0) as Hincl'.
+        eapply normalize_reset_wc_env in H1...
+        rewrite Hck. repeat constructor.
+        eapply wc_exp_clockof in H7...
+        rewrite H8 in H7; inv H7. rewrite <- app_assoc in H10.
+        repeat solve_incl. apply incl_app; [repeat solve_incl|].
+        unfold st_clocks. apply incl_map...
+      + repeat solve_incl.
+  Qed.
+
+  Corollary normalize_rhss_wc_eq : forall G vars es keep_fby es' eqs' st st',
+      wc_global G ->
+      wc_env (vars++st_clocks st) ->
+      Forall (wc_exp G (vars++st_clocks st)) es ->
+      normalize_rhss keep_fby es st = (es', eqs', st') ->
+      Forall (wc_equation G (vars++st_clocks st')) eqs' /\
+      wc_env (vars++st_clocks st').
+  Proof with eauto.
+    intros G vars es keep_fby es' eqs' st st' HwG Hwenv Hwc Hnorm.
+    unfold normalize_rhss in Hnorm; repeat inv_bind.
+    eapply map_bind2_wc_eq in H...
+    solve_forall.
+    eapply normalize_rhs_wc_eq with (G:=G) (vars:=vars) in H4...
+    repeat solve_incl.
+  Qed.
+
+  Fact normalize_equation_wc_eq : forall G vars e to_cut eqs' st st',
+      wc_global G ->
+      wc_env (vars++st_clocks st) ->
+      wc_equation G (vars++st_clocks st) e ->
+      normalize_equation to_cut e st = (eqs', st') ->
+      Forall (wc_equation G (vars++st_clocks st')) eqs' /\
+      wc_env (vars++st_clocks st').
+  Proof with eauto.
+    intros G vars [xs es] to_cut eqs' st st' HwG Hwenv Hwc Hnorm.
+    unfold normalize_equation in Hnorm. repeat inv_bind.
+    destruct Hwc as [Hwc1 [Hwc2 Hwc3]].
+    assert (st_follows st st') as Hfollows by eauto.
+    assert (H':=H). eapply normalize_rhss_wc_eq in H' as [Hwc' Hwenv']...
+    split...
+    apply Forall_app; split...
+    rewrite clocksof_nclocksof, Forall2_map_2 in Hwc3.
+    eapply Forall2_Forall2 in Hwc2; [|eapply Hwc3]. clear Hwc3.
+    replace (nclocksof es) with (nclocksof x) in Hwc2.
+    2: { eapply normalize_rhss_nclocksof in H... }
+    eapply normalize_rhss_wc_exp in H... clear Hwc1 Hwc' Hwenv'.
+    revert xs H Hwc2.
+    induction x; intros xs Hwc1 Hwc2; simpl in *; constructor.
+    + inv Hwc1.
+      assert (length (firstn (numstreams a) xs) = length (nclockof a)) as Hlen1.
+      { apply Forall2_length in Hwc2. rewrite app_length in Hwc2.
+        rewrite firstn_length, Hwc2, length_nclockof_numstreams.
+        apply Nat.min_l. omega. }
+      rewrite <- (firstn_skipn (numstreams a) xs) in Hwc2.
+      apply Forall2_app_split in Hwc2 as [Hwc2 _]...
+      repeat constructor...
+      * simpl. rewrite app_nil_r.
+        eapply Forall2_impl_In... intros; simpl in *. destruct H3...
+      * simpl. rewrite app_nil_r, clockof_nclockof, Forall2_map_2.
+        eapply Forall2_impl_In... intros; simpl in *. destruct H3...
+        apply in_or_app. apply in_app_or in H3. destruct H3...
+        right. eapply st_follows_clocks_incl...
+    + inv Hwc1. apply IHx...
+      assert (length (firstn (numstreams a) xs) = length (nclockof a)) as Hlen1.
+      { apply Forall2_length in Hwc2. rewrite app_length in Hwc2.
+        rewrite firstn_length, Hwc2, length_nclockof_numstreams.
+        apply Nat.min_l. omega. }
+      rewrite <- (firstn_skipn (numstreams a) xs) in Hwc2.
+      apply Forall2_app_split in Hwc2 as [_ Hwc2]...
+  Qed.
+
+  Corollary normalize_equations_wc_eq : forall G vars eqs to_cut eqs' st st',
+      wc_global G ->
+      wc_env (vars++st_clocks st) ->
+      Forall (wc_equation G (vars++st_clocks st)) eqs ->
+      normalize_equations to_cut eqs st = (eqs', st') ->
+      Forall (wc_equation G (vars++st_clocks st')) eqs' /\
+      wc_env (vars++st_clocks st').
+  Proof with eauto.
+    induction eqs; intros to_cut eqs' st st' HwG Hwenv Hwc Hnorm;
+      simpl in *; repeat inv_bind...
+    assert (st_follows st x0) as Hfollows1 by repeat solve_st_follows.
+    assert (st_follows x0 st') as Hfollows2 by repeat solve_st_follows.
+    inv Hwc. eapply normalize_equation_wc_eq in H as [Hwc1 Hwenv1]...
+    apply IHeqs in H0 as [Hwc2 Hwenv2]... 2:solve_forall; repeat solve_incl.
+    split...
+    apply Forall_app; split...
+    solve_forall; repeat solve_incl.
+  Qed.
+
+  Lemma normalize_node_wc : forall G n to_cut Hwl n',
+      wc_global G ->
+      wc_node G n ->
+      normalize_node to_cut n Hwl = n' ->
+      wc_node G n'.
+  Proof with eauto.
+    intros G n to_cut Hwl n' HwG [Hin [Hout [Henv Heq]]] Hnorm.
+    unfold normalize_node in Hnorm. subst.
+    repeat constructor; simpl; auto.
+    - remember (normalize_equations _ _ _) as res. symmetry in Heqres.
+      destruct res as [eqs' st']; simpl.
+      unfold idck. repeat rewrite map_app.
+      eapply normalize_equations_wc_eq in Heqres as [_ Henv']...
+      2,3:unfold st_clocks; rewrite init_st_anns, app_nil_r...
+      2:rewrite (Permutation_app_comm (n_vars _)) in Heq...
+      unfold idck in Henv'; repeat rewrite map_app in Henv'; repeat rewrite <- app_assoc in Henv'...
+    - remember (normalize_equations _ _ _) as res. symmetry in Heqres.
+      destruct res as [eqs' st']; simpl.
+      unfold idck. repeat rewrite map_app.
+      eapply normalize_equations_wc_eq in Heqres as [Hwc' _]...
+      2,3:unfold st_clocks; rewrite init_st_anns, app_nil_r...
+      2:rewrite (Permutation_app_comm (n_vars _)) in Heq...
+      unfold idck in Hwc'; repeat rewrite map_app in Hwc'; repeat rewrite <- app_assoc in *.
+      rewrite (Permutation_app_comm (map _ (idty _))), (Permutation_swap (map _ (n_vars _)))...
+  Qed.
+
+  Lemma normalize_global_wc : forall G Hwl G',
+      wc_global G ->
+      normalize_global G Hwl = G' ->
+      wc_global G'.
+  Proof.
+    induction G; intros Hwl G' Hwt Hnorm; simpl in Hnorm; inv Hwt.
+    - constructor.
+    - constructor.
+      + eapply IHG; eauto.
+      + remember (normalize_node _ _ _) as n'. symmetry in Heqn'.
+        eapply normalize_node_wc in Heqn'; eauto. simpl in Heqn'.
+        eapply iface_eq_wc_node; eauto.
+        eapply normalize_global_eq.
+      + eapply normalize_global_names; eauto.
+  Qed.
 End NCLOCKING.
 
 Module NClockingFun
